add syntax for contract definition

main/Semantics.v
@@ -1,5 +1,7 @@
 Require Import main.Syntax.
+
 Open Scope list_scope.
+
 Import ListNotations.
 
 
@@ -9,23 +11,56 @@ Import ListNotations.
 Definition EnvStack := list (FunctionEnv * ContractState).
 
 Definition ExecutionState : Type :=  Code * FunctionEnv * EnvStack * ContractState * ContractsEnv * Balance_Env.
+Definition CompileState : Type :=  contract_parts * ContractState.
+
+Inductive compile_step : CompileState -> CompileState -> Prop :=
+| function_definition:
+    forall name body rest c_st c_st',
+      c_st' = replace_contract_fn_env c_st (defineFunction (fn_env c_st) name (Body body)) ->
+      compile_step (Define_Function name body :: rest, c_st)
+                   (rest, c_st)
+
+| declare_aexp_fields:
+    forall aexp_env' aexp_names rest c_st c_st',
+      aexp_env' = declareAexpList (aexp_vars c_st) aexp_names ->
+      c_st' = replace_contract_aexp_env c_st aexp_env' ->
+      compile_step ((Declare_Aexp_Fields aexp_names) :: rest, c_st)
+                   (rest, c_st')
+
+| define_aexp_field:
+    forall aexp_env' aexp_def rest c_st c_st',
+      aexp_env' = defineAexp (aexp_vars c_st) aexp_def ->
+      c_st' = replace_contract_aexp_env c_st aexp_env' ->
+      compile_step ((Define_Aexp_Field aexp_def) :: rest, c_st)
+                   (rest, c_st')
+
+| declare_bexp_fields:
+    forall bexp_env' bexp_names rest c_st c_st',
+      bexp_env' = declareBexpList (bexp_vars c_st) bexp_names ->
+      c_st' = replace_contract_bexp_env c_st bexp_env' ->
+      compile_step ((Declare_Bexp_Fields bexp_names) :: rest, c_st)
+               (rest, c_st')
+
+| define_bexp_field:
+    forall bexp_env' bexp_def rest c_st c_st',
+      bexp_env' = defineBexp (bexp_vars c_st) bexp_def ->
+      c_st' = replace_contract_bexp_env c_st bexp_env' ->
+      compile_step ((Define_Bexp_Field bexp_def) :: rest, c_st) 
+                   (rest, c_st').
 
 
 (**************************************************************)
 (** Big Step Transitions *)
 
-Inductive step : ExecutionState -> ExecutionState -> Prop :=
+Inductive run_step : ExecutionState -> ExecutionState -> Prop :=
 | transfer:
     forall dest_addr amount value final_bm rest fenv env_stack c_st c_env new_bm src_addr bm,
       src_addr = (c_address c_st) ->
       value = unfold_option_z (eval_aexp (aexp_env fenv) bm amount) ->
       new_bm = (updateBalance bm dest_addr (unfold_option_z (bm dest_addr) + value)) ->
       final_bm = (updateBalance new_bm src_addr (unfold_option_z (new_bm src_addr) - value)) ->
-      step (Transfer dest_addr amount :: rest, fenv, env_stack, c_st, c_env, bm)
-           (rest,
-           fenv,
-           env_stack,
-           c_st, c_env, final_bm)
+      run_step (Transfer dest_addr amount :: rest, fenv, env_stack, c_st, c_env, bm)
+           (rest, fenv, env_stack, c_st, c_env, final_bm)
 
 | function_call:
     forall called_addr msg_val value env env_stack c_st c_env c_st' fenv fcode fname rest bm,
@@ -33,33 +68,37 @@ Inductive step : ExecutionState -> ExecutionState -> Prop :=
       fcode = getFunctionCode ((fn_env c_st') fname) ->
       value = unfold_option_z (eval_aexp (aexp_env env) bm (unfold_option msg_val Default_Aexp)) ->
       fenv = mkEnv (aexp_vars c_st') (bexp_vars c_st') (rest) (mkMsg value (c_address c_st)) ->
-      step ((Function_Call called_addr fname msg_val) :: rest, env, env_stack, c_st, c_env, bm) 
+      run_step ((Function_Call called_addr fname msg_val) :: rest, env, env_stack, c_st, c_env, bm) 
            (fcode, fenv, (env, c_st) :: env_stack, c_st', c_env, bm)
 
 | function_exit:
     forall (fenv fenv' : FunctionEnv) (c_st c_st' : ContractState) env_stack c_env bm,
-      step (nil, fenv, (fenv', c_st') :: env_stack, c_st, c_env, bm)
+      run_step (nil, fenv, (fenv', c_st') :: env_stack, c_st, c_env, bm)
            (next_code fenv', fenv', env_stack, c_st', c_env, bm)
 
 | skip:
     forall rest env env_stack c_st c_env bm,
-      step (Skip :: rest, env, env_stack, c_st, c_env, bm) (rest, env, env_stack, c_st, c_env, bm)
+      run_step (Skip :: rest, env, env_stack, c_st, c_env, bm) (rest, env, env_stack, c_st, c_env, bm)
 
-(** aexp declaration and assignment *)
+(** aexp var declaration *)
 
 | declare_aexp_local:
     forall aexp_env' aexp_names rest env env' env_stack c_st c_env bm,
       aexp_env' = declareAexpList (aexp_env env) aexp_names ->
       env' = mkEnv aexp_env' (bexp_env env) (next_code env) (msg_data env) ->
-      step ((Declare_Aexp aexp_names) :: rest, env, env_stack, c_st, c_env, bm) 
+      run_step ((Declare_Aexp aexp_names) :: rest, env, env_stack, c_st, c_env, bm)
             (rest, env', env_stack, c_st, c_env, bm)
 
-| declare_aexp_contract:
-    forall aexp_env' aexp_names rest env env_stack c_st c_st' c_env bm,
-      aexp_env' = declareAexpList (aexp_vars c_st) aexp_names ->
-      c_st' = replace_contract_aexp_env c_st aexp_env' ->
-      step ((Declare_Aexp aexp_names) :: rest, env, env_stack, c_st, c_env, bm) 
-            (rest, env, env_stack, c_st', c_env, bm)
+(** aexp var definition *)
+
+| define_aexp_local:
+    forall aexp_env' aexp_def rest env env' env_stack c_st c_env bm,
+      aexp_env' = defineAexp (aexp_env env) aexp_def ->
+      env' = mkEnv aexp_env' (bexp_env env) (next_code env) (msg_data env) ->
+      run_step ((Define_Aexp aexp_def) :: rest, env, env_stack, c_st, c_env, bm)
+            (rest, env', env_stack, c_st, c_env, bm)
+
+(** aexp assignment *)
 
 | assign_aexp_local :
     forall a x v aexp_env' rest env env' env_stack c_st c_env string_id bm,
@@ -67,7 +106,7 @@ Inductive step : ExecutionState -> ExecutionState -> Prop :=
       v = unfold_option_z (eval_aexp (aexp_env env) bm a) ->
       aexp_env' = update_aexp (aexp_env env) string_id v ->
       env' = mkEnv aexp_env' (bexp_env env) (next_code env) (msg_data env) ->
-      step (Assignment_Aexp x a :: rest, env, env_stack, c_st, c_env, bm) 
+      run_step (Assign_Aexp x a :: rest, env, env_stack, c_st, c_env, bm) 
            (rest, env', env_stack, c_st, c_env, bm)
 
 | assign_aexp_contract :
@@ -78,24 +117,28 @@ Inductive step : ExecutionState -> ExecutionState -> Prop :=
       contract_aexp_env = update_aexp (aexp_vars c_st) string_id v ->
       env' = mkEnv local_aexp_env (bexp_env env) (next_code env) (msg_data env) ->
       c_st' = replace_contract_aexp_env c_st contract_aexp_env ->
-      step (Assignment_Aexp x a :: rest, env, env_stack, c_st, c_env, bm) 
+      run_step (Assign_Aexp x a :: rest, env, env_stack, c_st, c_env, bm) 
            (rest, env', env_stack, c_st', c_env, bm)
 
-(** bexp declaration and assignment *)
+(** bexp var declaration *)
 
 | declare_bexp_local:
     forall bexp_env' bexp_names rest env env' env_stack c_st c_env bm,
       bexp_env' = declareBexpList (bexp_env env) bexp_names ->
       env' = mkEnv (aexp_env env) bexp_env' (next_code env) (msg_data env) ->
-      step ((Declare_Bexp bexp_names) :: rest, env, env_stack, c_st, c_env, bm) 
+      run_step ((Declare_Bexp bexp_names) :: rest, env, env_stack, c_st, c_env, bm) 
             (rest, env', env_stack, c_st, c_env, bm)
 
-| declare_bexp_contract:
-    forall bexp_env' bexp_names rest env env_stack c_st c_st' c_env bm,
-      bexp_env' = declareBexpList (bexp_vars c_st) bexp_names ->
-      c_st' = replace_contract_bexp_env c_st bexp_env' ->
-      step ((Declare_Bexp bexp_names) :: rest, env, env_stack, c_st, c_env, bm) 
-            (rest, env, env_stack, c_st', c_env, bm)
+(** bexp var definition *)
+
+| define_bexp_local:
+    forall bexp_env' bexp_def rest env env' env_stack c_st c_env bm,
+      bexp_env' = defineBexp (bexp_env env) bexp_def ->
+      env' = mkEnv (aexp_env env) bexp_env' (next_code env) (msg_data env) ->
+      run_step ((Define_Bexp bexp_def) :: rest, env, env_stack, c_st, c_env, bm) 
+            (rest, env', env_stack, c_st, c_env, bm)
+
+(** bexp assignment *)
 
 | assign_bexp_local :
     forall b x v bexp_env' rest env env' env_stack c_st c_env bm string_id,
@@ -103,7 +146,7 @@ Inductive step : ExecutionState -> ExecutionState -> Prop :=
       v = unfold_option_bool (eval_bexp (aexp_env env) bm (bexp_env env) b) ->
       bexp_env' = update_bexp (bexp_env env) string_id v ->
       env' = mkEnv (aexp_env env) (bexp_env') (next_code env) (msg_data env) ->
-      step (Assignment_Bexp x b :: rest, env, env_stack, c_st, c_env, bm) 
+      run_step (Assign_Bexp x b :: rest, env, env_stack, c_st, c_env, bm) 
            (rest, env', env_stack, c_st, c_env, bm)
 
 | assign_bexp_contract :
@@ -114,7 +157,7 @@ Inductive step : ExecutionState -> ExecutionState -> Prop :=
       contract_bexp_env = update_bexp (bexp_vars c_st) string_id v ->
       env' = mkEnv (aexp_env env) local_bexp_env (next_code env) (msg_data env) ->
       c_st' = replace_contract_bexp_env c_st contract_bexp_env ->
-      step (Assignment_Bexp x b :: rest, env, env_stack, c_st, c_env, bm) 
+      run_step (Assign_Bexp x b :: rest, env, env_stack, c_st, c_env, bm) 
            (rest, env', env_stack, c_st', c_env, bm)
 
 (** if *)
@@ -122,20 +165,20 @@ Inductive step : ExecutionState -> ExecutionState -> Prop :=
 | if_true :
     forall b s1 s2 rest env env_stack c_st c_env bm,
       Some true = (eval_bexp (aexp_env env) bm (bexp_env env) b) ->
-      step (IfThenElse b s1 s2 :: rest, env, env_stack, c_st, c_env, bm) 
+      run_step (IfThenElse b s1 s2 :: rest, env, env_stack, c_st, c_env, bm) 
            (s1 ++ rest, env, env_stack, c_st, c_env, bm)
 
 | if_false :
     forall b s1 s2 rest env env_stack c_st c_env bm,
       Some false = (eval_bexp (aexp_env env) bm (bexp_env env) b) ->
-      step (IfThenElse b s1 s2 :: rest, env, env_stack, c_st, c_env, bm)
+      run_step (IfThenElse b s1 s2 :: rest, env, env_stack, c_st, c_env, bm)
            (s2 ++ rest, env, env_stack, c_st, c_env, bm)
 
 (** while *)
 
 | while:
     forall (s : list instr) b rest env env_stack c_st c_env bm,
-      step (While b s :: rest, env, env_stack, c_st, c_env, bm)
+      run_step (While b s :: rest, env, env_stack, c_st, c_env, bm)
            ([IfThenElse b (s ++ (While b s :: rest)) rest], env, env_stack, c_st, c_env, bm)
 .
 
@@ -143,11 +186,23 @@ Inductive step : ExecutionState -> ExecutionState -> Prop :=
 (**************************************************************)
 (** Binary relations on steps *)
 
-Inductive steps : ExecutionState -> ExecutionState -> Prop :=
-| refl : forall S,
-    steps S S
-| trans: forall S S' S'',
-    step S S' -> steps S' S'' -> steps S S''.
+Inductive compile_steps : CompileState -> CompileState -> Prop :=
+| compile_refl : forall S,
+    compile_steps S S
+| compile_trans: forall S S' S'',
+    compile_step S S' -> compile_steps S' S'' -> compile_steps S S''.
+
+Inductive run_steps : ExecutionState -> ExecutionState -> Prop :=
+| run_refl : forall S,
+    run_steps S S
+| run_trans: forall S S' S'',
+    run_step S S' -> run_steps S' S'' -> run_steps S S''.
+
+
+
+(* Theorem transfer_correct: forall  next_step,
+  steps transfer next_step ->  *)
+
 
 
 (**************************************************************)
@@ -167,15 +222,15 @@ Let example_contracts_env := Empty_ContractsEnv.
 Let new_balances := (updateBalance (updateBalance Empty_BalanceEnv receiver amount_z) (c_address Default_ContractState) (-amount_z)).
 
 Example transfer_ex:
-  steps (Transfer receiver amount_aexp :: nil, Empty_FunctionEnv, nil, Default_ContractState, example_contracts_env, Empty_BalanceEnv)
+  run_steps (Transfer receiver amount_aexp :: nil, Empty_FunctionEnv, nil, Default_ContractState, example_contracts_env, Empty_BalanceEnv)
         (nil, Empty_FunctionEnv, nil, Default_ContractState, example_contracts_env, new_balances).
 Proof.
-  eapply trans.
+  eapply run_trans.
   {
     eapply transfer; eauto.
   }
   {
-    apply refl.
+    apply run_refl.
   }
   Qed.
 
@@ -187,7 +242,7 @@ End transfer.
 
 Section function_call.
 
-Let called_fn_code := [Declare_Aexp [("fn_a", None)]].
+Let called_fn_code := [Declare_Aexp ["fn_a"]].
 Let called_fn := "called_fn".
 Let called_contract_funs_env := defineFunction Empty_Functions_Env called_fn (Body called_fn_code).
 Let called_contract_address := "called_contract".
@@ -199,22 +254,22 @@ Let example_contracts_env := updateContractsEnv Empty_ContractsEnv called_contra
 
 Let msg_val := Int 0.
 Let msg_val_z := 0.
-Let current_vars : list (string * option aexp) := [("a", None)].
+Let current_vars := ["a"].
 Let current_code := (Declare_Aexp current_vars) :: (Function_Call (Some called_contract_address) called_fn (Some msg_val)) :: nil.
 
 Let fn_env_before_call := (replace_aexp_env Empty_FunctionEnv (declareAexpList (aexp_env Empty_FunctionEnv) current_vars)).
 Let called_fn_env := replace_msg_data Empty_FunctionEnv (mkMsg  msg_val_z (c_address calling_contract_state)).
 
 Example Step_Into_Call :
-  steps (current_code, Empty_FunctionEnv, nil, calling_contract_state, example_contracts_env, Empty_BalanceEnv)
+  run_steps (current_code, Empty_FunctionEnv, nil, calling_contract_state, example_contracts_env, Empty_BalanceEnv)
         (called_fn_code, called_fn_env, (fn_env_before_call, calling_contract_state) :: nil,
          called_contract_state, example_contracts_env, Empty_BalanceEnv).
 Proof.
-  eapply trans.
+  eapply run_trans.
   - eapply declare_aexp_local; eauto.
-  - eapply trans.
+  - eapply run_trans.
     * eapply function_call; eauto.
-    * apply refl.
+    * apply run_refl.
 Qed.
 
 End function_call.
@@ -236,17 +291,17 @@ Let example_contracts_env := updateContractsEnv
 Default_Address calling_contract_state.
 
 Example Function_exit:
-  steps (nil, Empty_FunctionEnv, (fenv_with_remaining_code, calling_contract_state)::nil,
+  run_steps (nil, Empty_FunctionEnv, (fenv_with_remaining_code, calling_contract_state)::nil,
   called_contract_state, example_contracts_env, Empty_BalanceEnv)
   (next_code fenv_with_remaining_code, fenv_with_remaining_code, nil,
    calling_contract_state, example_contracts_env, Empty_BalanceEnv).
 Proof.
-  eapply trans.
+  eapply run_trans.
   {
     eapply function_exit; eauto.
   }
   {
-    apply refl.
+    apply run_refl.
   }
   Qed.
 
@@ -258,11 +313,11 @@ End function_exit.
 
 Section contract_and_local_var.
 
-Let called_fn_code := [Declare_Aexp [("local_a", Some (Int 100))]; Assignment_Aexp (AId "contract_a") (AId "local_a")].
+Let called_fn_code := [Define_Aexp ("local_a", Int 100); Assign_Aexp (AId "contract_a") (AId "local_a")].
 Let called_fn := "called_fn".
 Let called_contract_funs_env := defineFunction Empty_Functions_Env called_fn (Body called_fn_code).
 Let called_contract_address := "called_contract".
-Let contract_aexp_env := declareAexpList Empty_Aexp_Env [("contract_a", None)].
+Let contract_aexp_env := declareAexpList Empty_Aexp_Env ["contract_a"].
 Let called_contract_state := 
 mkContractState called_contract_address called_contract_funs_env contract_aexp_env Empty_Bexp_Env.
 Let final_contract_state :=
@@ -272,16 +327,16 @@ Let final_fn_env :=
 replace_aexp_env initial_fn_env (update_aexp (update_aexp contract_aexp_env (Some "local_a") 100) (Some "contract_a") 100).
 
 Example contract_and_local_var:
-steps (called_fn_code, initial_fn_env, [], called_contract_state, Empty_ContractsEnv, Empty_BalanceEnv)
+run_steps (called_fn_code, initial_fn_env, [], called_contract_state, Empty_ContractsEnv, Empty_BalanceEnv)
       ([], final_fn_env, [], final_contract_state, Empty_ContractsEnv, Empty_BalanceEnv).
 Proof.
-  eapply trans.
+  eapply run_trans.
   {
-    eapply declare_aexp_local; eauto.
+    eapply define_aexp_local; eauto.
   }
-  eapply trans.
+  eapply run_trans.
   eapply assign_aexp_contract; eauto.
-  eapply refl.
+  eapply run_refl.
 Qed.
 
 End contract_and_local_var.
@@ -309,30 +364,30 @@ Let funs_env_Alice := defineFunction Empty_Functions_Env fun_name_Alice (Body fu
 Let contract_Alice := mkContractState address_Alice funs_env_Alice Empty_Aexp_Env Empty_Bexp_Env.
 
 Example Looped_Transfer:
-steps (fun_code_Alice, Empty_FunctionEnv, [], contract_Alice, Empty_ContractsEnv, initial_balances)
+run_steps (fun_code_Alice, Empty_FunctionEnv, [], contract_Alice, Empty_ContractsEnv, initial_balances)
       ([], Empty_FunctionEnv, [], contract_Alice, Empty_ContractsEnv, final_balances).
 Proof.
-  eapply trans.
+  eapply run_trans.
   {
     eapply while; eauto.
   }
-  eapply trans.
+  eapply run_trans.
   {  
     eapply if_true; eauto.
   }
-  eapply trans.
+  eapply run_trans.
   {
     eapply transfer; eauto.
   }
-  eapply trans.
+  eapply run_trans.
   {
     eapply while; eauto.
   }
-  eapply trans.
+  eapply run_trans.
   {  
     eapply if_false; eauto.
   }
-  apply refl.
+  apply run_refl.
 Qed.
 
 End looped_transfer.
