main/Syntax.v
@@ -5,6 +5,7 @@ Require Export List.
 Open Scope string_scope.
 Open Scope Z_scope.
 
+Import ListNotations.
 
 (**************************************************************)
 (** Solidity address *)
@@ -31,6 +32,7 @@ Inductive aexp :=
 | Int : Z -> aexp
 | AId : string -> aexp
 | Plus : aexp -> aexp -> aexp
+| Sub : aexp -> aexp -> aexp
 | Mul : aexp -> aexp -> aexp
 | Div : aexp -> aexp -> aexp
 | Rem : aexp -> aexp -> aexp
@@ -48,6 +50,7 @@ Inductive bexp :=
 | Aexp_Lt : aexp -> aexp -> bexp
 | Aexp_Leq : aexp -> aexp -> bexp
 | Aexp_Eq : aexp -> aexp -> bexp
+| Aexp_Neq : aexp -> aexp -> bexp
 | Aexp_Geq : aexp -> aexp -> bexp
 | Aexp_Gt : aexp -> aexp -> bexp
 | Not : bexp -> bexp
@@ -73,16 +76,39 @@ Definition Default_Msg := {| value := 0;
 (** Statements *)
 
 Inductive instr :=
-| Declare_Aexp : list (string * option aexp) -> instr
-| Declare_Bexp : list (string * option bexp) -> instr
-| Assignment_Aexp : aexp -> aexp -> instr
-| Assignment_Bexp : bexp -> bexp -> instr
+| Declare_Aexp : list string -> instr
+| Declare_Bexp : list string -> instr
+
+| Define_Aexp : (string * aexp) -> instr
+| Define_Bexp : (string * bexp) -> instr
+
+| Assign_Aexp : aexp -> aexp -> instr
+| Assign_Bexp : bexp -> bexp -> instr
+
 | IfThenElse : bexp -> list instr -> list instr -> instr
 | While : bexp -> list instr -> instr
 | Skip : instr
+
 (* no params, no return value, with value setter *)
 | Function_Call : option address -> string -> option aexp -> instr (* "this" "f" Some Int value *)
 | Transfer : address_payable -> aexp -> instr.
+
+
+Inductive contract_part :=
+| Define_Function : string -> list instr -> contract_part
+
+| Declare_Aexp_Fields : list string -> contract_part
+| Declare_Bexp_Fields : list string -> contract_part
+
+| Define_Aexp_Field : (string * aexp) -> contract_part
+| Define_Bexp_Field : (string * bexp) -> contract_part.
+
+
+Definition contract_parts := list contract_part.
+
+
+(* Notation "'uint' id = v" := (Declare_Aexp (id, Some (Int v)) :: rest)
+  (at level 200). *)
 
 
 (**************************************************************)
@@ -194,6 +220,11 @@ Definition replace_contract_bexp_env :=
 fun (cstate : ContractState) (new_env : Bexp_Env)
  => mkContractState (c_address cstate) (fn_env cstate) (aexp_vars cstate) new_env.
 
+Definition replace_contract_fn_env := 
+fun (cstate : ContractState) (new_env : Functions_Env)
+ => mkContractState (c_address cstate) new_env (aexp_vars cstate) (bexp_vars cstate).
+
+
 Definition Default_ContractState := {| c_address := Default_Address;
                                        fn_env := Empty_Functions_Env;
                                        aexp_vars := Empty_Aexp_Env;
@@ -268,18 +299,63 @@ end.
 (**************************************************************)
 (** Declaration helpers *)
 
-Fixpoint declareAexpList (env : Aexp_Env) (decl_pairs : list (string * option aexp)) : Aexp_Env :=
+(* Fixpoint declareAexpList (env : Aexp_Env) (decl_pairs : list (string * option aexp)) : Aexp_Env :=
 fun x => match decl_pairs with
 | nil => env x
-| decl :: rest => if (string_dec x (fst decl)) then 
+| decl :: rest => if (string_dec x (fst decl)) then
                       match (snd decl) with
                       | None => unfold_aexp_literal Default_Aexp
                       | Some v => unfold_aexp_literal v
                       end
                   else declareAexpList env rest x
+end. *)
+
+
+Fixpoint declareAexpList (env : Aexp_Env) (id_list : list string) : Aexp_Env :=
+fun x => match id_list with
+| nil => env x
+| id :: rest => if (string_dec x id) then unfold_aexp_literal Default_Aexp
+                else declareAexpList env rest x
 end.
 
-Fixpoint declareBexpList (env : Bexp_Env) (decl_pairs : list (string * option bexp)) : Bexp_Env :=
+(** [TEST] declareAexpList *)
+
+Let env := update_aexp Empty_Aexp_Env (Some "x") 1.
+Compute (declareAexpList env ["y"; "x"]) "x".
+
+(***************************)
+
+Definition defineAexp (env : Aexp_Env) (def : string * aexp) : Aexp_Env :=
+fun x => match def with
+| (id, Int v) => if (string_dec x id) then Some v
+                 else env x
+| (_, _) => env x
+end.
+
+(** [TEST] defineAexp *)
+
+Let env1 := update_aexp Empty_Aexp_Env (Some "x") 1.
+Compute (defineAexp env1 ("z", Int 33)) "z".
+Compute (defineAexp env1 ("z", AId "x")) "z".
+
+(***************************)
+
+
+Fixpoint declareBexpList (env : Bexp_Env) (id_list : list string) : Bexp_Env :=
+fun x => match id_list with
+| nil => env x
+| id :: rest => if (string_dec x id) then unfold_bexp_literal Default_Bexp
+                else declareBexpList env rest x
+end.
+
+Definition defineBexp (env : Bexp_Env) (def : string * bexp) : Bexp_Env :=
+fun x => match def with
+| (id, Boolean v) => if (string_dec x id) then Some v
+                 else env x
+| (_, _) => env x
+end.
+
+(* Fixpoint declareBexpList (env : Bexp_Env) (decl_pairs : list (string * option bexp)) : Bexp_Env :=
 fun x => match decl_pairs with
 | nil => env x
 | decl :: rest => if (string_dec x (fst decl)) then 
@@ -289,6 +365,7 @@ fun x => match decl_pairs with
                       end
                   else declareBexpList env rest x
 end.
+ *)
 
 
 (**************************************************************)
@@ -303,6 +380,10 @@ Fixpoint eval_aexp (env : Aexp_Env) (bm : Balance_Env) (a : aexp) : option Z :=
   | BalanceOf x => bm x
   | Plus a1 a2 => match (eval_aexp env bm a1), (eval_aexp env bm a2) with
                   | Some v1, Some v2 => Some (Z.add v1 v2)
+                  | _, _ => None
+                  end
+  | Sub a1 a2 => match (eval_aexp env bm a1), (eval_aexp env bm a2) with
+                  | Some v1, Some v2 => Some (Z.sub v1 v2)
                   | _, _ => None
                   end
   | Mul a1 a2 => match (eval_aexp env bm a1), (eval_aexp env bm a2) with
@@ -364,6 +445,10 @@ Fixpoint eval_bexp (aexp_env : Aexp_Env) (bm : Balance_Env) (bexp_env : Bexp_Env
                     end
   | Aexp_Eq a1 a2 => match (eval_aexp aexp_env bm a1), (eval_aexp aexp_env bm a2) with
                     | Some v1, Some v2 => Some (Z.eqb v1 v2)
+                    | _, _ => None
+                    end
+  | Aexp_Neq a1 a2 => match (eval_aexp aexp_env bm a1), (eval_aexp aexp_env bm a2) with
+                    | Some v1, Some v2 => Some (Zneq_bool v1 v2)
                     | _, _ => None
                     end
   | Aexp_Geq a1 a2 => match (eval_aexp aexp_env bm a1), (eval_aexp aexp_env bm a2) with
